TotalAlgebra.thy
@@ -1,0 +1,219 @@
+theory TotalAlgebra
+imports TotalStateUtil Viper.SepAlgebra
+begin
+
+
+subsection \<open>Addition and multiplication of total states\<close>
+
+text \<open>Total states are compatible only if their heaps are the same.\<close>
+definition compatible_pre_total :: "'a pre_total_state \<Rightarrow> 'a pre_total_state \<Rightarrow> bool"
+  where
+    "compatible_pre_total \<phi>1 \<phi>2 =    
+         ( get_h_pre_total \<phi>1 = get_h_pre_total \<phi>2 \<and>
+           wf_mask_simple (add_masks (get_mh_pre_total \<phi>1) (get_mh_pre_total \<phi>2)))"
+
+definition pre_plus_total :: "'a pre_total_state \<Rightarrow> 'a pre_total_state \<Rightarrow> 'a pre_total_state option" where
+  "pre_plus_total \<phi>1 \<phi>2 =
+    (if compatible_pre_total \<phi>1 \<phi>2 then
+       Some (get_h_pre_total \<phi>1, 
+            ( add_masks (get_mh_pre_total \<phi>1) (get_mh_pre_total \<phi>2),
+              add_masks (get_mp_pre_total \<phi>1) (get_mp_pre_total \<phi>2)))
+     else None)"
+
+definition compatible_total :: "'a total_state \<Rightarrow> 'a total_state \<Rightarrow> bool"
+  where
+    "compatible_total \<phi>1 \<phi>2 =    
+         ( get_h_total \<phi>1 = get_h_total \<phi>2 \<and>
+           wf_mask_simple (add_masks (get_mh_total \<phi>1) (get_mh_total \<phi>2)))"
+
+fun add_m_total :: "mask \<times> 'a predicate_mask \<Rightarrow> mask \<times> 'a predicate_mask \<Rightarrow> mask \<times> 'a predicate_mask"
+  where "add_m_total m1 m2 = (add_masks (fst m1) (fst m2), add_masks (snd m1) (snd m2))"
+
+definition plus_total :: "'a total_state \<Rightarrow> 'a total_state \<Rightarrow> 'a total_state option" (infixl "|\<oplus>|\<^sub>t" 60)  where
+  "\<phi>1 |\<oplus>|\<^sub>t \<phi>2 =
+    (if compatible_total \<phi>1 \<phi>2 then
+        Some (update_m_total \<phi>1 (add_m_total (get_m_total \<phi>1) (get_m_total \<phi>2) ) 
+             )
+     else None)"
+
+lemma comm_compatible_pre_total: "compatible_pre_total \<phi>1 \<phi>2 = compatible_pre_total \<phi>2 \<phi>1"
+  unfolding compatible_pre_total_def
+  by (auto simp: add_masks_comm)
+
+lemma comm_compatible_total: "compatible_total \<phi>1 \<phi>2 = compatible_total \<phi>2 \<phi>1"
+  unfolding compatible_total_def
+  by (auto simp: add_masks_comm)
+
+lemma pre_plus_total_wf : "pre_plus_total \<phi>1 \<phi>2 = Some \<phi>3  \<Longrightarrow> wf_mask_simple (get_mh_pre_total \<phi>3)"
+  unfolding pre_plus_total_def compatible_pre_total_def
+  by (auto split: if_split_asm)
+
+lemma pre_plus_total_same_h : "pre_plus_total \<phi>1 \<phi>2 = Some \<phi>3  \<Longrightarrow> get_h_pre_total \<phi>1 = get_h_pre_total \<phi>2"
+  unfolding pre_plus_total_def compatible_pre_total_def
+  by (auto split: if_split_asm)
+
+
+lemma comm_plus_total: "a |\<oplus>|\<^sub>t b = b |\<oplus>|\<^sub>t a"
+  unfolding plus_total_def
+  by (simp split: if_split add: add_masks_comm compatible_total_def update_m_total_def)
+
+lemma plus_total_defined_h_eq_1:
+  assumes "a |\<oplus>|\<^sub>t b = Some c"
+  shows "get_h_total a = get_h_total b"
+  using assms
+  unfolding plus_total_def
+  by (simp add:compatible_total_def split: if_split_asm)
+
+lemma plus_total_defined_h_eq_2:
+  assumes "a |\<oplus>|\<^sub>t b = Some c"
+  shows "get_h_total a = get_h_total c"
+  using assms
+  unfolding plus_total_def
+  apply (simp add:compatible_total_def split: if_split_asm)
+  by (metis fst_conv get_h_pre_total.simps get_h_total.simps get_h_update_m_total)
+
+lemma plus_total_m: 
+  assumes "\<phi>1 |\<oplus>|\<^sub>t \<phi>2 = Some \<phi>3"
+  shows "get_m_total \<phi>3 = (add_m_total (get_m_total \<phi>1) (get_m_total \<phi>2))"
+  using assms
+  unfolding plus_total_def
+  apply (simp split: if_split_asm del: get_mh_total.simps get_mp_total.simps get_m_total.simps)
+  using compatible_total_def get_m_update_m_total by fastforce
+
+
+lemma plus_total_defined: "a |\<oplus>|\<^sub>t b \<noteq> None \<longleftrightarrow> compatible_total a b"
+  unfolding plus_total_def
+  by (simp split: if_split)
+
+lemma assoc1_plus_total: 
+  assumes "a |\<oplus>|\<^sub>t b = Some ab" and "b |\<oplus>|\<^sub>t c = Some bc"
+  shows "ab |\<oplus>|\<^sub>t c = a |\<oplus>|\<^sub>t bc"
+proof -
+  from assms have Heq1: "get_h_total a = get_h_total b" "get_h_total b = get_h_total c"
+    by (simp_all only: plus_total_defined_h_eq_1 )
+  from assms have Heq2: "get_h_total a = get_h_total ab" "get_h_total b = get_h_total bc"
+    by (simp_all only: plus_total_defined_h_eq_2)
+  
+  from assms have Meq1: "get_m_total ab  = add_m_total (get_m_total a) (get_m_total b)"
+    by (simp only: plus_total_m)
+
+  from assms have Meq2: "get_m_total bc  = add_m_total (get_m_total b) (get_m_total c)"
+    by (simp only: plus_total_m)
+
+  show ?thesis
+  proof (cases "ab |\<oplus>|\<^sub>t c = None")
+  case True
+    hence "\<not> compatible_total ab c"
+      using plus_total_defined by blast
+    hence "\<not> wf_mask_simple (add_masks (get_mh_total ab) (get_mh_total c))"
+      using Heq1 Heq2 compatible_total_def by fastforce
+    then show ?thesis
+      using Meq1 Meq2 add_masks_assoc
+      by (metis (no_types, lifting) add_m_total.simps compatible_total_def fstI get_m_mh_mp_total plus_total_def)
+next
+  case False
+  hence "compatible_total ab c"
+      using plus_total_defined by blast
+  hence "compatible_total a bc"
+    unfolding compatible_total_def
+      using Heq1 Heq2 Meq1 Meq2 add_masks_assoc
+      by (metis add_m_total.simps fst_conv get_mh_from_m_total) 
+    from this obtain y where PEq1: "a |\<oplus>|\<^sub>t bc = Some y"
+      using plus_total_defined by blast
+     from \<open>ab |\<oplus>|\<^sub>t c \<noteq> None\<close> obtain x where PEq2:"ab |\<oplus>|\<^sub>t c = Some x"
+      using plus_total_defined by blast
+    have "x = y"
+      apply (rule total_state_eq)           
+       apply (subst plus_total_m[OF PEq1])
+       apply (subst plus_total_m[OF PEq2])
+       apply (subst Meq1)
+       apply (subst Meq2)
+       apply (simp add: add_masks_assoc)
+      by (metis Heq2(1) PEq1 PEq2 plus_total_defined_h_eq_2)
+    thus ?thesis
+      by (simp add: PEq1 PEq2)
+  qed
+qed
+
+lemma assoc2_plus_total:
+  assumes "a |\<oplus>|\<^sub>t b = Some ab" and "b |\<oplus>|\<^sub>t c = None"
+  shows "ab |\<oplus>|\<^sub>t c = None"
+proof -
+  from assms(2) have "\<not> compatible_total b c"
+    using plus_total_defined by blast
+  hence "get_h_total b \<noteq> get_h_total c \<or> \<not> wf_mask_simple (add_masks (get_mh_total b) (get_mh_total c))"
+    by (simp add: compatible_total_def)
+  thus ?thesis
+  proof
+    assume "get_h_total b \<noteq> get_h_total c"
+    hence "get_h_total c \<noteq> get_h_total ab"
+      using assms(1) plus_total_defined_h_eq_1 plus_total_defined_h_eq_2
+      by fastforce
+    thus "ab |\<oplus>|\<^sub>t c = None"
+      by (simp add: compatible_total_def plus_total_def)
+  next
+    assume "\<not> wf_mask_simple (add_masks (get_mh_total b) (get_mh_total c))"
+    hence "\<not> wf_mask_simple (add_masks (add_masks (get_mh_total a) (get_mh_total b)) (get_mh_total c))"
+      using wf_mask_simple_false_preserved add_masks_comm add_masks_assoc
+      by metis
+    thus ?thesis
+      using plus_total_m assms(1)
+      by (metis (no_types, lifting) add_m_total.elims compatible_total_def fstI get_mh_from_m_total plus_total_defined)
+  qed
+qed
+
+lemma assoc3_plus_total:
+  assumes "a |\<oplus>|\<^sub>t b = None" and "b |\<oplus>|\<^sub>t c = Some bc"
+  shows "a |\<oplus>|\<^sub>t bc = None"
+  using assms comm_plus_total assoc2_plus_total
+  by metis
+
+text \<open>Multiplication of states (TODO: duplication in Viper.EquiViper)\<close>
+definition mult_mask :: "prat \<Rightarrow> mask \<Rightarrow> mask" where
+  "mult_mask p \<pi> x = pmult p (\<pi> x)"
+
+definition multiplicable_mask :: "prat \<Rightarrow> mask \<Rightarrow> bool" where
+  "multiplicable_mask p \<pi> \<longleftrightarrow> (\<forall>hl. lte (pmult p (\<pi> hl)) pwrite)"
+
+definition update_mh_total :: "'a total_state \<Rightarrow> mask \<Rightarrow> 'a total_state"
+  where "update_mh_total \<phi> mh = Abs_total_state (get_h_total \<phi>, (mh, get_mp_total \<phi>))"
+
+definition mult_total :: "prat \<Rightarrow> 'a total_state \<Rightarrow> 'a total_state option" (infixl "|\<odot>|\<^sub>t" 70) where
+  "\<alpha> |\<odot>|\<^sub>t \<phi> = (if multiplicable_mask \<alpha> (get_mh_total \<phi>) then 
+                   Some (update_mh_total \<phi> (mult_mask \<alpha> (get_mh_total \<phi>))) else None
+               )"
+
+definition core_total :: "'a total_state \<Rightarrow> 'a total_state"
+  where "core_total \<phi> = update_m_total \<phi> (zero_mask, zero_mask)"
+
+lemma add_core_total: "x |\<oplus>|\<^sub>t core_total x = Some x"
+  unfolding core_total_def plus_total_def
+  apply (simp split: if_split del: get_m_total.simps)
+  apply (rule conjI)
+   apply (rule impI)
+   apply (metis (no_types, hide_lams) compatible_total_def fst_conv get_h_update_m_total get_m_mh_mp_total get_m_update_m_total snd_conv total_state_eq wf_zero_mask zero_mask_neutral)
+  apply (unfold compatible_total_def)
+  apply (rule conjI)
+   apply (metis fst_conv get_h_update_m_total wf_zero_mask)
+  apply (unfold wf_mask_simple_def)
+  by (metis fst_conv get_m_update_m_total get_mask_total_wf get_mh_from_m_total wf_mask_simple_def wf_zero_mask zero_mask_neutral)
+
+definition stable_total :: "'a total_state \<Rightarrow> bool"
+  where "stable_total _ = True"
+
+definition stabilize_total :: "'a total_state \<Rightarrow> 'a total_state"
+  where "stabilize_total = id"
+
+global_interpretation TotalViper: sep_algebra plus_total mult_total core_total stable_total stabilize_total
+  unfolding sep_algebra_def
+  apply (intro conjI)
+              apply (simp add: comm_plus_total)
+             apply (blast intro: assoc1_plus_total)
+            apply (blast intro: assoc2_plus_total)
+           apply (blast intro: assoc3_plus_total)
+          apply (blast intro: HOL.sym[OF add_core_total])
+
+
+  
+
+end
