TotalStateUtil.thy
@@ -1,0 +1,247 @@
+theory TotalStateUtil
+imports TotalViperState
+begin
+
+section \<open>update_store_total\<close>
+
+fun update_var_total :: "'a full_total_state \<Rightarrow> var \<Rightarrow> 'a val \<Rightarrow> 'a full_total_state"
+  where "update_var_total \<omega> x v = ((get_store_total \<omega>)(x \<mapsto> v), get_trace_total \<omega>, get_total_full \<omega>)"
+
+lemma update_var_total_trace_eq: "get_trace_total (update_var_total \<omega> x v) = get_trace_total \<omega>"
+  by simp
+
+lemma update_var_total_hm_same: "get_total_full (update_var_total \<omega> x v) = get_total_full \<omega>"
+  by simp
+
+lemma update_var_total_heap_same: "get_hh_total_full (update_var_total \<omega> x v) = get_hh_total_full \<omega>"
+  by simp
+
+lemma update_var_total_mask_same: "get_total_full (update_var_total \<omega> x v) = get_total_full \<omega>"
+  by simp
+
+fun update_store_total :: "'a full_total_state \<Rightarrow> 'a store \<Rightarrow> 'a full_total_state"
+  where "update_store_total \<omega> \<sigma> = (\<sigma>, get_trace_total \<omega>, get_total_full \<omega>)"
+
+section \<open>update_trace_total\<close>
+
+fun update_trace_total :: "'a full_total_state \<Rightarrow> 'a total_trace \<Rightarrow> 'a full_total_state"
+  where "update_trace_total \<omega> \<pi> = (get_store_total \<omega>, \<pi>, get_total_full \<omega>)"
+
+lemma update_trace_total_store_same: "get_store_total (update_trace_total \<omega> \<pi>) = get_store_total \<omega>"
+  by simp
+
+lemma update_trace_total_hm_same: "get_total_full (update_trace_total \<omega> \<pi>) = get_total_full \<omega>"
+  by simp
+
+lemma update_trace_total_heap_same: "get_hh_total_full (update_trace_total \<omega> \<pi>) = get_hh_total_full \<omega>"
+  by simp
+
+lemma update_trace_total_mask_same: "get_mh_total_full (update_trace_total \<omega> \<pi>) = get_mh_total_full \<omega>"
+  by simp
+
+section \<open>update heap and mask total\<close>
+
+definition update_hh_loc_total :: "'a total_state \<Rightarrow> heap_loc \<Rightarrow> 'a val \<Rightarrow> 'a total_state"
+  where "update_hh_loc_total \<phi> l v = Abs_total_state (((get_hh_total \<phi>)(l := v), get_hp_total \<phi>), get_m_total \<phi>)"
+
+definition update_mh_total :: "'a total_state \<Rightarrow> mask \<Rightarrow> 'a total_state"
+  where "update_mh_total \<phi> mh = Abs_total_state (get_h_total \<phi>, (mh, get_mp_total \<phi>))"
+
+definition update_mp_total :: "'a total_state \<Rightarrow> 'a predicate_mask \<Rightarrow> 'a total_state"
+  where "update_mp_total \<phi> mp = Abs_total_state (get_h_total \<phi>, (get_mh_total \<phi>, mp))"
+
+definition update_m_total :: "'a total_state \<Rightarrow> mask \<times> 'a predicate_mask \<Rightarrow> 'a total_state"
+  where "update_m_total \<phi> m = Abs_total_state (get_h_total \<phi>, m)"
+
+
+lemma Abs_total_state_inverse_2:
+  assumes "wf_pre_total_state (m,h)"
+  shows "Rep_total_state (Abs_total_state (m,h)) = (m,h)"
+  using assms Abs_total_state_inverse
+  by blast
+
+lemma get_m_update_m_total:
+  assumes "wf_mask_simple (fst m)"
+  shows "get_m_total (update_m_total \<phi> m) = m"
+  unfolding update_m_total_def
+  using assms
+  by (simp add: Abs_total_state_inverse_2)
+
+
+lemma get_h_update_m_total:
+  assumes "wf_mask_simple (fst m)"
+  shows "get_h_total (update_m_total \<phi> m) = get_h_total \<phi>"
+  unfolding update_m_total_def
+  using assms
+  by (simp add: Abs_total_state_inverse_2)            
+
+lemma update_m_total_eq: 
+  assumes "wf_mask_simple (fst m)" and
+          "get_h_total \<phi>1 = get_h_total \<phi>2"
+  shows "update_m_total \<phi>1 m = update_m_total \<phi>2 m"
+  apply (rule total_state_eq)
+   apply (simp only: get_m_update_m_total[OF assms(1)])
+  apply (simp only: get_h_update_m_total[OF assms(1)] assms(2))
+  done
+  
+lemma get_update_mh_total: 
+  assumes "wf_mask_simple m0"
+  shows   "get_mh_total (update_mh_total mh m0) = m0"
+  unfolding update_mh_total_def
+  using assms
+  by (simp add: Abs_total_state_inverse_2)
+
+lemma update_mh_total_multiple: 
+  assumes "wf_mask_simple m0" and "wf_mask_simple m2"
+  shows   "update_mh_total (update_mh_total mh m0) m1 = update_mh_total mh m1"
+  unfolding update_mh_total_def  
+  using assms
+  by (simp add: Abs_total_state_inverse_2)
+
+lemma wf_pre_total_state_1: 
+  assumes"get_mh_pre_total \<phi>' = get_mh_total \<phi>"
+  shows "wf_pre_total_state \<phi>'"
+  using assms
+  using get_mask_total_wf by fastforce
+
+lemma update_hh_loc_total_m_eq: "get_m_total (update_hh_loc_total \<phi> l v) = get_m_total \<phi>"
+  unfolding update_hh_loc_total_def
+proof -
+  let ?\<phi>' = "(((get_hh_total \<phi>)(l := v), get_hp_total \<phi>), get_m_total \<phi>)"
+  have "wf_pre_total_state ?\<phi>'"
+    apply (rule wf_pre_total_state_1[where ?\<phi>=\<phi>])
+    by simp
+  thus "get_m_total (Abs_total_state ?\<phi>') = (get_m_total \<phi>)"
+    by (simp add: Abs_total_state_inverse_2)
+qed
+
+lemma m_eq_mh_eq_total: "get_m_total \<phi> = get_m_total \<phi>' \<Longrightarrow> get_mh_total \<phi> = get_mh_total \<phi>'"
+  by simp
+
+lemma m_eq_mp_eq_total: "get_m_total \<phi> = get_m_total \<phi>' \<Longrightarrow> get_mp_total \<phi> = get_mp_total \<phi>'"
+  by simp
+
+lemma update_hh_loc_total_mh_eq: "get_mh_total (update_hh_loc_total \<phi> l v) = get_mh_total \<phi>"
+  using m_eq_mh_eq_total update_hh_loc_total_m_eq
+  by blast
+
+lemma update_hh_loc_total_mp_eq: "get_mp_total (update_hh_loc_total \<phi> l v) = get_mp_total \<phi>"
+  using m_eq_mp_eq_total update_hh_loc_total_m_eq
+  by blast
+
+lemma update_hh_loc_total_hp_eq: "get_hp_total (update_hh_loc_total \<phi> l v) = get_hp_total \<phi>"
+  unfolding update_hh_loc_total_def
+proof -
+  let ?\<phi>' = "(((get_hh_total \<phi>)(l := v), get_hp_total \<phi>), get_m_total \<phi>)"
+  have "wf_pre_total_state ?\<phi>'"
+    apply (rule wf_pre_total_state_1[where ?\<phi>=\<phi>])
+    by simp
+  thus "get_hp_total (Abs_total_state ?\<phi>') = (get_hp_total \<phi>)"
+    by (simp add: Abs_total_state_inverse_2)
+qed
+
+lemma Rep_total_state_inj: "Rep_total_state a = Rep_total_state b \<Longrightarrow> a = b"
+  by (metis Rep_total_state_inverse)
+
+lemma update_hh_loc_total_fupd: "get_hh_total (update_hh_loc_total \<phi> l1 v) = (get_hh_total \<phi>)(l1 := v)"
+  unfolding update_hh_loc_total_def
+proof -
+  let ?\<phi>'="(((get_hh_total \<phi>)(l1 := v), get_hp_total \<phi>), get_m_total \<phi>)"
+  have "wf_pre_total_state ?\<phi>'"
+    apply (rule wf_pre_total_state_1[where ?\<phi>=\<phi>])
+    by simp
+  thus "get_hh_total (Abs_total_state ?\<phi>') = (get_hh_total \<phi>)(l1 := v)"
+    by (simp add: Abs_total_state_inverse_2)
+qed
+
+lemma update_hh_loc_total_lookup_1: "get_hh_total (update_hh_loc_total \<phi> l v) l = v"
+  using update_hh_loc_total_fupd
+  by (metis fun_upd_same)
+
+lemma update_hh_loc_total_lookup_2: "l1 \<noteq> l2 \<Longrightarrow> get_hh_total (update_hh_loc_total \<phi> l1 v) l2 = get_hh_total \<phi> l2"
+  using update_hh_loc_total_fupd
+  by (metis fun_upd_apply)
+
+lemma update_hh_loc_total_overwrite: "update_hh_loc_total (update_hh_loc_total \<phi> l v1) l v2 = update_hh_loc_total \<phi> l v2"
+proof -  
+  let ?\<phi>' = "update_hh_loc_total \<phi> l v1"
+  let ?\<phi>'' = "update_hh_loc_total ?\<phi>' l v2"
+  let ?\<phi>_rhs = "update_hh_loc_total \<phi> l v2"
+  have "get_hh_total ?\<phi>'' = (get_hh_total \<phi>)(l := v2)"
+    by (metis fun_upd_upd update_hh_loc_total_fupd)
+  hence A:"get_hh_total ?\<phi>'' = get_hh_total (update_hh_loc_total \<phi> l v2)"
+    by (metis update_hh_loc_total_fupd)
+  show ?thesis
+    apply (rule total_state_eq)
+     apply (simp only: update_hh_loc_total_m_eq)
+    apply (rule total_heap_eq)
+     apply (rule A)
+    apply (simp only: update_hh_loc_total_hp_eq)
+    done
+qed
+
+fun update_hh_loc_total_full :: "'a full_total_state \<Rightarrow> heap_loc \<Rightarrow> 'a val \<Rightarrow> 'a full_total_state"
+  where "update_hh_loc_total_full \<omega> l v = (get_store_total \<omega>, get_trace_total \<omega>, update_hh_loc_total (get_total_full \<omega>) l v )"
+
+lemma update_hh_loc_total_full_lookup_1: "get_hh_total_full (update_hh_loc_total_full \<phi> l v) l = v"
+  by (metis get_hh_total_full.simps get_total_full.simps snd_conv update_hh_loc_total_full.simps update_hh_loc_total_lookup_1)
+
+lemma update_hh_loc_total_full_lookup_2: "l1 \<noteq> l2 \<Longrightarrow> get_hh_total_full (update_hh_loc_total_full \<phi> l1 v) l2 = get_hh_total_full \<phi> l2"
+  by (metis get_hh_total_full.simps get_total_full.simps snd_conv update_hh_loc_total_full.simps update_hh_loc_total_lookup_2)
+
+lemma update_hh_loc_total_overwrite_full: "update_hh_loc_total_full (update_hh_loc_total_full \<omega> l v1) l v2 = update_hh_loc_total_full \<omega> l v2"
+  oops
+  
+fun update_mh_total_full :: "'a full_total_state \<Rightarrow> mask \<Rightarrow> 'a full_total_state"
+  where "update_mh_total_full \<omega> mh = (get_store_total \<omega>, get_trace_total \<omega>, update_mh_total (get_total_full \<omega>) mh)"
+
+fun update_mp_total_full :: "'a full_total_state \<Rightarrow> 'a predicate_mask \<Rightarrow> 'a full_total_state"
+  where "update_mp_total_full \<omega> mp = (get_store_total \<omega>, get_trace_total \<omega>, update_mp_total (get_total_full \<omega>) mp)"
+
+lemma update_hh_loc_total_full_mask_same: "get_mh_total_full (update_hh_loc_total_full \<omega> l v) = get_mh_total_full \<omega>"
+  by (metis get_total_full.simps get_mh_total_full.simps snd_conv update_hh_loc_total_full.simps update_hh_loc_total_mh_eq)
+
+lemma get_update_mh_total_full: 
+  assumes "wf_mask_simple m0"
+  shows   "get_mh_total_full (update_mh_total_full mh m0) = m0"
+  using assms get_update_mh_total
+  by auto
+
+lemma update_mh_total_full_same:
+  "(update_mh_total_full \<omega> (get_mh_total_full \<omega>)) = \<omega>"
+  by (simp add: update_mh_total_def Rep_total_state_inverse)
+
+lemma update_mp_total_h_eq: 
+  shows "get_h_total (update_mp_total \<phi> m) = get_h_total \<phi>"
+  by (metis Abs_total_state_inverse_2 fst_conv get_h_pre_total.simps get_h_total.elims get_m_pre_total.simps get_mask_total_wf snd_conv update_mp_total_def wf_pre_total_state.simps)
+
+lemma update_mp_total_h_full_eq: 
+  shows "get_h_total_full (update_mp_total_full \<phi> m) = get_h_total_full \<phi>"
+  using update_mp_total_h_eq
+  by auto
+
+lemma update_mh_total_h_eq: 
+  assumes "wf_mask_simple m"
+  shows "get_h_total (update_mh_total \<phi> m) = get_h_total \<phi>"
+  unfolding update_mh_total_def
+  using assms
+  by (simp add: Abs_total_state_inverse)
+
+lemma update_mh_total_full_hh_eq: 
+  assumes "wf_mask_simple m"
+  shows "get_h_total_full (update_mh_total_full \<phi> m) = get_h_total_full \<phi>"
+  using assms update_mh_total_h_eq
+  by auto
+
+lemma update_mh_total_full_multiple: 
+  assumes "wf_mask_simple m0"
+  shows   "update_mh_total_full (update_mh_total_full \<omega> m0) m1 = update_mh_total_full \<omega> m1"
+  using assms
+  using update_mh_total_multiple by fastforce
+
+fun update_m_total_full :: "'a full_total_state \<Rightarrow> mask \<Rightarrow> 'a predicate_mask \<Rightarrow> 'a full_total_state"
+  where "update_m_total_full \<omega> m pm = 
+                (get_store_total \<omega>, get_trace_total \<omega>, 
+                 update_mp_total (update_mh_total (get_total_full \<omega>) m) pm)"
+
+end
